---
title: 201709304
date: 2017-09-30
categories: MATH
tags: [ç½—å°”å®šç†]
banner: http://ox0p9pctg.bkt.clouddn.com/201709304.jpeg
thumbnail: http://ox0p9pctg.bkt.clouddn.com/201709304.jpeg
---

#### é¢˜ 4:

è®¾ f(x) åœ¨[0,1] ä¸Šæœ‰äºŒé˜¶å¯¼æ•°ï¼Œf(0)=f(1)=f'(0)=f'(1)=0ï¼Œè¯æ˜å­˜åœ¨ ğ›âˆˆ(0,1)ï¼Œä½¿å¾—f''(ğ›)=f(ğ›).

<!--more-->

- - -

#### è¯æ˜

æ„é€ è¾…åŠ©å‡½æ•° $F(x)=[f(x)+f'(x)]e^{-x}$.

ç”±é¢˜è®¾å¯çŸ¥F(x)åœ¨[0,1]ä¸Šè¿ç»­ï¼Œåœ¨(0,1)å¯å¯¼ï¼Œä¸”F(0)=F(1).ç”±ç½—å°”å®šç†å¯çŸ¥è‡³å°‘å­˜åœ¨ä¸€ç‚¹ ğ›âˆˆ(0,1)ï¼Œä½¿å¾—F'(ğ›)=0.

åˆ $F'(x)=[f'(x)+f''(x)]e^{-x}-[f(x)+f'(x)]e^{-x}=[f''(x)-f(x)]e^{-x}$.ç”±äº $e^{-x}\neq0ï¼Œå¯çŸ¥æœ‰f''(ğ›)-f(ğ›)=0ï¼Œå³f''(ğ›)=f(ğ›).$

- - -
THE END.
